lift the type of cbor_det_serialize_tag

src/cbor/pulse/CBOR.Pulse.API.Base.fst
@@ -1507,3 +1507,27 @@ let cbor_free_t
   stt unit
     (freeable x)
     (fun _ -> emp)
+
+noextract [@@noextract_to "krml"]
+let cbor_det_serialize_tag_postcond
+  (tag: U64.t)
+  (output: S.slice U8.t)
+  (res: SZ.t)
+  (v': Seq.seq U8.t)
+: Tot prop
+= let s = Spec.cbor_det_serialize_tag tag in
+  let len = Seq.length s in
+  SZ.v (S.len output) == Seq.length v' /\
+  (res == 0sz <==> len > Seq.length v') /\
+  (len <= Seq.length v' ==> Seq.slice v' 0 len == s)
+
+inline_for_extraction
+let cbor_det_serialize_tag_t =
+  (tag: U64.t) ->
+  (output: S.slice U8.t) ->
+  stt SZ.t
+    (exists* v . pts_to output v)
+    (fun res -> exists* v . pts_to output v ** pure (
+      cbor_det_serialize_tag_postcond tag output res v
+    ))
+
